tutorial/Imp.v
@@ -2,16 +2,21 @@
 
 (** We now demonstrate how to use ITrees in the context of verified compilation.
     To this end, we will consider a simple compiler from an imperative language
-    to a control-flow-graph language.
-    The meaning of both languages will be given in terms of ITrees, so that the
-    proof of correctness is expressed by proving a bisimulation between ITrees.
-    We shall emphasize two main satisfying aspects of the resulting formalization.
+    to a control-flow-graph language.  The meaning of both languages will be
+    given in terms of ITrees, so that the proof of correctness is expressed by
+    proving a bisimulation between ITrees.
+
+    We shall emphasize two main satisfying aspects of the resulting
+    formalization.
+
     - Despite the correctness being termination-sensitive, we do not write any
-    cofixpoints. All reasoning is purely equational, and the underlying
-    coinductive reasoning is hidden on the library side.
-    - We split the correctness in two steps. First, a linking theory of the CFG language
-    is proved correct. Then, this theory is leveraged to prove the functional correctness
-    of the compiler. The first piece is fairly generic, and hence reusable.
+      cofixpoints. All reasoning is purely equational, and the underlying
+      coinductive reasoning is hidden on the library side.
+
+    - We split the correctness in two steps. First, a linking theory of the CFG
+      language is proved correct. Then, this theory is leveraged to prove the
+      functional correctness of the compiler. The first piece is fairly generic,
+      and hence reusable.
  *)
 
 (** This tutorial is composed of the following files:
@@ -21,15 +26,15 @@
     - AsmCombinators.v     : Linking theory for Asm
     - Imp2Asm.v            : Compiler from Imp to Asm
     - Imp2AsmCorrectness.v : Proof of correctness of the compiler
+    - AsmOptimizations.v   : (Optional) optimization passes for the Asm language
     The intended entry point for reading is Imp.v.
  *)
 
-(** We therefore start by introducing a simplified variant of Software Foundations'
-    [Imp] language.
-    The language's semantics is first expressed in terms of [itree]s.
-    The semantics of the program can then be obtained by
-    interpreting the events contained in the trees.
- *)
+(** We therefore start by introducing a simplified variant of Software
+    Foundations' [Imp] language.  The language's semantics is first expressed in
+    terms of [itree]s.  The semantics of the program can then be obtained by
+    interpreting the events contained in the trees.  
+*)
 
 (* begin hide *)
 From Coq Require Import
@@ -58,7 +63,7 @@ Local Open Scope monad_scope.
 Local Open Scope string_scope.
 (* end hide *)
 
-(* ================================================================= *)
+(* ========================================================================== *)
 (** ** Syntax *)
 
 (** Imp manipulates a countable set of variables represented as [string]s: *)
@@ -86,7 +91,7 @@ Inductive stmt : Type :=
 | Skip                           (* ; *)
 .
 
-(* ================================================================= *)
+(* ========================================================================== *)
 (** ** Notations *)
 
 Module ImpNotations.
@@ -133,7 +138,7 @@ End ImpNotations.
 
 Import ImpNotations.
 
-(* ================================================================= *)
+(* ========================================================================== *)
 (** ** Semantics *)
 
 (** _Imp_ produces effects by manipulating its variables.  To account for this,
@@ -183,11 +188,13 @@ Section Denote.
 
   (** We turn to the denotation of statements. As opposed to expressions,
       statements do not return any value: their semantic domain is therefore
-      [itree eff unit]. The most interesting construct is naturally [while].
+      [itree eff unit]. The most interesting construct is, naturally, [while].
 
       To define its meaning, we make use of the [loop] combinator provided by
       the [itree] library:
+
       [loop : (C + A -> itree E (C + B)) -> A -> itree E B].
+
       The combinator takes as argument the body of the loop, i.e. a function
       that maps inputs of type [C + A] to an [itree] computing either a [C] that
       can be fed back to the loop, or a return value of type [B]. The combinator
@@ -195,14 +202,14 @@ Section Denote.
       
       Compared to the [mrec] and [rec] combinators introduced in
       [Introduction.v], [loop] is more restricted in that it naturally
-      represents tail recursive functions.
-      It however enjoys a rich equational theory: its addition grants the type
-      of _continuation trees_, named [ktree]s in the library, a structure of
-      _traced monoidal category_.
+      represents tail recursive functions.  It however enjoys a rich equational
+      theory: its addition grants the type of _continuation trees_ (named
+      [ktree]s in the library), a structure of a _traced monoidal category_.
 
-      We use [loop] to first build a new combinator [while] that takes a step
-      of the loop (i.e. the loop guard 
-   *)
+      We use [loop] to first build a new combinator [while] that takes a step of
+      the loop (i.e. the loop guard The "control" behavior of the loop is
+      governed by a value of type [unit + unit].  The right tag [inr tt] says to
+      exit the loop, and the [inl tt] says to continue.  *)
 
   Definition while {eff} (step : itree eff (unit + unit)) : itree eff unit :=
     loop 
@@ -212,14 +219,15 @@ Section Denote.
          | inr _ => ret (inl tt)
          end) tt.
 
-  (** Casting values into [bool]. *)
+      
+  (** Casting values into [bool]:  [0] corresponds to [false] and any nonzero
+      value corresponds to [true].  *)
   Definition is_true (v : value) : bool := if (v =? 0)%nat then false else true.
 
-  (** The meaning of statements is now easy to define.
-      They are all straightforward, except for [While] that uses our new
-      [while] combinator over the computation that evaluates the conditional,
-      and then the body if the former was true.
-   *)
+  (** The meaning of statements is now easy to define.  They are all
+      straightforward, except for [While], whic uses our new [while] combinator
+      over the computation that evaluates the conditional, and then the body if
+      the former was true.  *)
   Fixpoint denote_stmt (s : stmt) : itree eff unit :=
     match s with
     | Assign x e =>  v <- denote_expr e ;; trigger (SetVar x v)
@@ -239,12 +247,13 @@ Section Denote.
 
 End Denote.
 
-(* ================================================================= *)
+(* ========================================================================== *)
 (** ** EXAMPLE: Factorial *)
 
 Section Example_Fact.
 
-  (** We briefly illustrate the language by writing the traditional factorial. *)
+  (** We briefly illustrate the language by writing the traditional factorial. 
+      example.  *)
 
   Open Scope expr_scope.
   Open Scope stmt_scope.
@@ -260,14 +269,13 @@ Section Example_Fact.
 
   (** We have given _a_ notion of denotation to [fact 6] via [denote_stmt].
       However this is naturally not actually runnable yet, since it contains
-      uninterpreted [ImpState] events.
-      We therefore now need to _handle_ the events contained
-      in the trees, i.e. give a concrete interpretation of the environment.
-   *)
+      uninterpreted [ImpState] events.  We therefore now need to _handle_ the
+      events contained in the trees, i.e. give a concrete interpretation of the
+      environment.  *)
 
 End Example_Fact.
 
-(* ================================================================= *)
+(* ========================================================================== *)
 (** ** Interpretation *)
 
 (* begin hide *)
@@ -293,16 +301,14 @@ Proof.
 Qed.
 (* end hide *)
 
-(** We provide an _ITree event handler_ to interpret away [ImpState] events.
-    We use an _environment event_ to do so, modeling the environment as
-    a 0-initialized environment.
-    Recall from [Introduction.v] that a _handler_ for the events [ImpState]
-    is a function of type [forall R, ImpState R -> M R] for some monad [M].
-    Here we take for our monad the special case of [M = itree E] for some
-    universe of events [E] required to contain the environment events [mapE]
-    provided by the library. It comes with an event handler [run_map]
-    interpreting the computation into the state monad.
- *)
+(** We provide an _ITree event handler_ to interpret away [ImpState] events.  We
+    use an _environment event_ to do so, modeling the environment as a
+    0-initialized map from strings to values.  Recall from [Introduction.v] that
+    a _handler_ for the events [ImpState] is a function of type [forall R, ImpState R
+    -> M R] for some monad [M].  Here we take for our monad the special case of
+    [M = itree E] for some universe of events [E] required to contain the
+    environment events [mapE] provided by the library. It comes with an event
+    handler [run_map] interpreting the computation into the state monad.  *)
 Definition eval_imp_state {E: Type -> Type} `{mapE var value -< E}: ImpState ~> itree E :=
   fun _ e =>
     match e with
@@ -327,17 +333,16 @@ Definition interp_imp  {E A} (t : itree (ImpState +' E) A) (g:globals) :=
   run_map t' g.
 
 
-Definition ImpEval (s: stmt) : itree void1 (globals * unit) :=
+Definition eval_imp (s: stmt) : itree void1 (globals * unit) :=
   interp_imp (denote_stmt s) empty.
 
 (** Equipped with this evaluator, we can now compute.
     Naturally since Coq is total, we cannot do it directly inside of it.
     We can either rely on extraction, or use some fuel.
  *)
-Compute (burn 200 (ImpEval (fact "x" "y" 6))). 
+Compute (burn 200 (eval_imp (fact "x" "y" 6))). 
 
-
-
+(* ========================================================================== *)
 Section InterpImpProperties.
   (** We can lift the underlying equational theory on [itree]s to include new
       equations for working with [interp_imp].  
@@ -348,9 +353,9 @@ Section InterpImpProperties.
 
       We could justify more equations than just the ones below.  For instance,
       _Imp_ programs also respect a coarser notation of equivalence for the 
-      [globals] state.
+      [globals] state.  We exploit this possibility to implement optimzations
+      at the _Asm_ level (see AsmOptimizations.v).
    *)
-
 
   Context {E': Type -> Type}.
   Notation E := (ImpState +' E').
